Set_Graphs/Directed_Graphs/Pair_Graph_RBT.thy
@@ -1,0 +1,42 @@
+theory Pair_Graph_RBT
+imports Pair_Graph_Specs "HOL-Data_Structures.RBT_Set" "HOL-Data_Structures.RBT_Map"
+       "Verified_SAT_Based_AI_Planning.Set2_Join_RBT"
+begin
+
+definition "neighb_inv \<equiv>  (\<lambda>t. (invc t \<and> invh t) \<and> Tree2.bst t)"
+
+fun sel where
+"sel Leaf = undefined" |
+"sel (B l a r) = a"|
+"sel (R l a r) = a"
+             
+interpretation set: Set Leaf insert_rbt delete_rbt isin Tree2.set_tree neighb_inv
+  apply unfold_locales
+  by (simp add: empty_def neighb_inv_def isin_set_tree RBT.set_isin RBT.set_tree_insert RBT.set_insert
+                RBT.set_tree_insert RBT.set_tree_delete RBT.set_delete RBT.set_delete 
+                RBT.invar_insert RBT.invar_insert RBT.invar_insert RBT.inv_delete RBT.invar_delete
+                RBT.inv_delete)+
+
+interpretation S_C: Set_Choose Leaf insert_rbt RBT.delete isin neighb_inv Tree2.set_tree sel
+  apply unfold_locales
+proof(goal_cases)
+  case (1 s)
+  then show ?case
+    by(induction rule: sel.induct) (auto simp: empty_def)
+qed
+
+interpretation G: Pair_Graph_Specs RBT_Set.empty RBT_Map.delete lookup insert_rbt isin Tree2.set_tree sel
+     update M.invar Leaf RBT.delete neighb_inv
+  apply(rule Pair_Graph_Specs.intro)
+  subgoal apply unfold_locales.
+  apply unfold_locales .
+
+fun fold_rbt where
+"fold_rbt f Leaf acc = acc"|
+"fold_rbt f (B l x r) acc= f x (fold_rbt f l (fold_rbt f r acc))"|
+"fold_rbt f (R l x r) acc= f x (fold_rbt f l (fold_rbt f r acc))"
+
+lemma fold_rbt_is_foldr_of_preorder:"fold_rbt f T acc = foldr f (map fst (preorder T)) acc "
+  by(induction f T acc arbitrary: rule: fold_rbt.induct) auto
+
+end
